almost there

utils/Zeta.MultiSet.SSeq.fst
@@ -96,19 +96,17 @@ let rec union_all (#a:eqtype) (#f: cmp a) (s: S.seq (mset a f))
   = if S.length s = 0 then
       empty
     else
-      let h = S.head s in
-      let s' = S.tail s in
-      union h (union_all s')
+      let prefix, last = S.un_snoc s in
+      union last (union_all prefix)
 
 let union_all_empty (#a: eqtype) (#f: cmp a) (s: S.seq (mset a f){ S.length s = 0 })
   : Lemma (ensures (union_all s == empty #a #f))
   = ()
 
-let union_all_cons (#a: eqtype) (#f: cmp a) (s: Seq.seq (mset a f) {Seq.length s > 0})
-  : Lemma (ensures (let tail = Seq.tail s in
-                    let hd = Seq.head s in
-                    union_all s == union hd (union_all tail)))
-  = ()
+let union_all_snoc (#a: eqtype) (#f: _) (s: Seq.seq (Zeta.MultiSet.mset a f) {Seq.length s > 0})
+  : Lemma (ensures (let prefix, last = Seq.un_snoc s in
+                    union_all s == Zeta.MultiSet.union last (union_all prefix)))
+  = ()                    
 
 let union_all_sseq (#a: eqtype) (#f: cmp a) (s: sseq a)
   : Lemma (ensures (let ms1: mset a f = sseq2mset s in
